Wavelet/Semantics.lean
@@ -4,5 +4,7 @@ import Wavelet.Semantics.Link
 import Wavelet.Semantics.OpInterp
 import Wavelet.Semantics.PCM
 import Wavelet.Semantics.Confluence
+import Wavelet.Semantics.Guard
+import Wavelet.Semantics.OpSpec
 
 /-! Common definitions for semantics. -/
