Wavelet/Semantics/Guard.lean
@@ -1,0 +1,135 @@
+import Wavelet.Semantics.Defs
+
+/-! Definitions to guard a semantics with a given state or label invariant. -/
+
+namespace Wavelet.Semantics
+
+/-- Restricts an LTS by imposing a state invariant. -/
+inductive Lts.GuardState {S} (Inv : S → Prop) (lts : Lts S E) : Lts S E where
+  | step : Inv s → Inv s' → lts.Step s e s' → GuardState Inv lts s e s'
+
+/-- Guards the transition of a semantics with the given invariant. -/
+def guardState
+  [Arity Op]
+  (sem : Semantics Op V m n)
+  (Inv : sem.S → Prop) :
+  Semantics Op V m n :=
+  {
+    S := sem.S,
+    init := sem.init,
+    lts := sem.lts.GuardState Inv,
+    -- TODO: this is actually not true,
+    -- maybe remove this requirement?
+    yields_functional := sorry
+  }
+
+/-- Modifies labels with a relation. -/
+inductive Lts.GuardLabel {S} (Guard : E → E' → Prop) (lts : Lts S E) : Lts S E' where
+  | step : Guard e e' → lts.Step s e s' → GuardLabel Guard lts s e' s'
+
+/-- Guards and interprets the labels as another set of operators. -/
+def guardLabel
+  [Arity Op] [Arity Op']
+  (sem : Semantics Op V m n)
+  (Guard : Label Op V m n → Label Op' V' m' n' → Prop) :
+  Semantics Op' V' m' n' :=
+  {
+    S := sem.S,
+    init := sem.init,
+    lts := sem.lts.GuardLabel Guard,
+    yields_functional := sorry
+  }
+
+/-- Combines `GuardState` and `GuardLabel`. -/
+def Lts.Guard {S}
+  (lts : Lts S E)
+  (Inv : S → Prop)
+  (Guard : E → E' → Prop) : Lts S E' :=
+  (lts.GuardState Inv).GuardLabel Guard
+
+/-- Combines `guardState` and `guardLabel`. -/
+def guard
+  [Arity Op] [Arity Op']
+  (sem : Semantics Op V m n)
+  (Inv : sem.S → Prop)
+  (Guard : Label Op V m n → Label Op' V' m' n' → Prop) :
+  Semantics Op' V' m' n' :=
+  (sem.guardState Inv).guardLabel Guard
+
+/-- Some well-formedness constraints on label guards. -/
+class LawfulLabelGuard [Arity Op] [Arity Op']
+  (Guard : Label Op V m n → Label Op' V' m' n' → Prop) where
+  label_guard_tau : Guard .τ .τ
+  label_guard_tau_only : ∀ {l}, Guard .τ l → l.isSilent
+  label_guard_input : ∀ {vals l}, Guard (.input vals) l → l.isSilent ∨ l.isInput
+  label_guard_output : ∀ {vals l}, Guard (.output vals) l → l.isSilent ∨ l.isOutput
+  label_guard_yield : ∀ {op inputs outputs l}, Guard (.yield op inputs outputs) l → l.isSilent ∨ l.isYield
+
+/-- Introduces a `Guard` step from a single step in the base LTS. -/
+theorem guard_single
+  {S : Type u}
+  {lts : Lts S E}
+  {Inv : S → Prop}
+  {Guard : E → E' → Prop}
+  {s s' : S}
+  (hstep : lts.Step s e s')
+  (hinv₁ : Inv s)
+  (hinv₂ : Inv s')
+  (hinterp : Guard e e') :
+  (lts.Guard Inv Guard).Step s e' s'
+:= by
+  apply Lts.GuardLabel.step hinterp
+  apply Lts.GuardState.step hinv₁ hinv₂ hstep
+
+/-- `guardLabel` preserves IO-restricted simulation. -/
+theorem sim_guard_label
+  [Arity Op] [Arity Op']
+  [DecidableEq χ]
+  [DecidableEq χ']
+  [InterpConsts V]
+  [InterpConsts V']
+  {sem₁ sem₂ : Semantics Op V m n}
+  {Guard : Label Op V m n → Label Op' V' m' n' → Prop}
+  [hguard : LawfulLabelGuard Guard]
+  (hsim : sem₁ ≲ᵣ sem₂) :
+  sem₁.guardLabel Guard ≲ᵣ sem₂.guardLabel Guard
+  := by
+  apply Lts.Similarity.intro hsim.Sim
+  constructor
+  · exact hsim.sim_init
+  · intros s₁ s₂ l s₁' hR hstep
+    simp [Semantics.guardLabel] at hstep
+    cases hstep with | step hlabel hstep =>
+    rename Label Op V m n => l'
+    have ⟨s₂', hstep_s₂, hR₂⟩ := hsim.sim_step _ _ _ _ hR hstep
+    exists s₂'
+    constructor
+    · cases hstep_s₂ with
+      | step_yield hstep_yield_s₂ =>
+        replace hstep_yield_s₂ := Lts.GuardLabel.step hlabel hstep_yield_s₂
+        cases hguard.label_guard_yield hlabel <;>
+          rename_i h₁ <;> cases l <;> simp at h₁
+        · exact .step_tau (.single hstep_yield_s₂)
+        · exact .step_yield hstep_yield_s₂
+      | step_input hstep_input_s₂ hstep_tau =>
+        replace hstep_input_s₂ := Lts.GuardLabel.step hlabel hstep_input_s₂
+        replace hstep_tau := hstep_tau.map (Lts.GuardLabel.step hguard.label_guard_tau)
+        cases hguard.label_guard_input hlabel <;>
+          rename_i h₁ <;> cases l <;> simp at h₁
+        · exact .step_tau (hstep_tau.prepend hstep_input_s₂)
+        · exact .step_input hstep_input_s₂ hstep_tau
+      | step_output hstep_tau hstep_output_s₂ =>
+        replace hstep_output_s₂ := Lts.GuardLabel.step hlabel hstep_output_s₂
+        replace hstep_tau := hstep_tau.map (Lts.GuardLabel.step hguard.label_guard_tau)
+        cases hguard.label_guard_output hlabel <;>
+          rename_i h₁ <;> cases l <;> simp at h₁
+        · exact .step_tau (hstep_tau.tail hstep_output_s₂)
+        · exact .step_output hstep_tau hstep_output_s₂
+      | step_tau hstep_tau_s₂ =>
+        replace hstep_tau_s₂ := hstep_tau_s₂.map (Lts.GuardLabel.step hguard.label_guard_tau)
+        have := hguard.label_guard_tau_only hlabel
+        cases l <;> simp at this
+        exact .step_tau hstep_tau_s₂
+    · exact hR₂
+
+end Wavelet.Semantics
