Wavelet/Semantics/OpSpec.lean
@@ -1,0 +1,139 @@
+import Wavelet.Semantics.Defs
+import Wavelet.Semantics.OpInterp
+import Wavelet.Semantics.Guard
+import Wavelet.Semantics.PCM
+import Wavelet.Semantics.Confluence
+
+/-! Putting a resource specification on an operator set. -/
+
+namespace Wavelet.Semantics
+
+/-- PCM specification of an operator set -/
+structure OpSpec Op V T [Arity Op] [PCM T] where
+  pre : (op : Op) → Vector V (Arity.ι op) → T
+  post : (op : Op) → Vector V (Arity.ι op) → Vector V (Arity.ω op) → T
+  frame_preserving : ∀ op inputs outputs, pre op inputs ⟹ post op inputs outputs
+
+/-- Two labels are compatible if their inputs correspond to disjoint resources
+and are deterministic. -/
+def OpSpec.CompatLabels
+  [Arity Op] [PCM T]
+  (opSpec : OpSpec Op V T) :
+  RespLabel Op V → RespLabel Op V → Prop
+  | .respond op₁ inputs₁ _, .respond op₂ inputs₂ _ =>
+    (opSpec.pre op₁ inputs₁) ⊥ (opSpec.pre op₂ inputs₂)
+
+def OpSpec.Sound
+  [Arity Op] [PCM T]
+  (opSpec : OpSpec Op V T)
+  (interp : OpInterp Op V) : Prop :=
+  ∀ s, interp.lts.StronglyConfluentAt s (OpSpec.CompatLabels opSpec)
+
+/-- Specification on input/output labels. -/
+structure IOSpec V T [PCM T] m n where
+  pre : Vector V m → T
+  -- This can only depend on the outputs, due
+  -- to a technical issue that we can't access
+  -- the input values at an output event.
+  post : Vector V n → T
+
+/-- Augments the operator set with an additional ghost argument
+to pass a PCM token, as well as two operators to split and join PCMs. -/
+inductive WithSpec (Op : Type u) [Arity Op] [PCM T] (spec : OpSpec Op V T) where
+  | op (op : Op)
+  | join (k : Nat) -- Number of input tokens to combine
+
+/-- Uses only the LHS `InterpConsts` of a sum for constants. -/
+instance instInterpConstsSum [left : InterpConsts V] : InterpConsts (V ⊕ V') where
+  junkVal := .inl (left.junkVal)
+  toBool
+    | .inl v => left.toBool v
+    | .inr _ => none
+  fromBool := .inl ∘ left.fromBool
+  unique_fromBool_toBool b := left.unique_fromBool_toBool b
+  unique_toBool_fromBool b v hv := by
+    split at hv
+    · rename_i v'
+      have := left.unique_toBool_fromBool b v' hv
+      simp [this]
+    · contradiction
+
+instance instArityWithSpec
+  [arity : Arity Op] [PCM T]
+  {spec : OpSpec Op V T} :
+  Arity (WithSpec Op spec) where
+  ι | .op o => arity.ι o + 1
+    | .join k => k
+  ω | .op o => arity.ω o + 1
+    | .join _ => 2
+
+/-- Interprets the labels with ghost values using the base operators,
+but with dynamic checks for ghost tokens satisfying the specs. -/
+inductive OpSpec.Guard
+  [Arity Op] [PCM T]
+  (opSpec : OpSpec Op V T)
+  (ioSpec : IOSpec V T m n) :
+  Label (WithSpec Op opSpec) (V ⊕ T) (m + 1) (n + 1) →
+  Label Op V m n → Prop where
+  | spec_yield
+    {op}
+    {inputs : Vector V (Arity.ι op)}
+    {outputs : Vector V (Arity.ω op)} :
+    tok₁ ≡ opSpec.pre op inputs →
+    tok₂ ≡ opSpec.post op inputs outputs →
+    Guard opSpec ioSpec
+      (.yield (.op op)
+        ((inputs.map .inl).push (.inr tok₁))
+        ((outputs.map .inl).push (.inr tok₂)))
+      (.yield op inputs outputs)
+  -- NOTE: the exact output split of permissions
+  -- is intentionally left unspecified, because
+  -- we want this to be dynamic without restricting
+  -- to a static annotation.
+  | spec_join
+    {toks : Vector T k}
+    {outputs : Vector (V ⊕ T) 2} :
+    outputs[0] = .inr tok₁ →
+    outputs[1] = .inr tok₂ →
+    tok₁ ⊔ tok₂ ≡ PCM.sum toks.toList →
+    Guard opSpec ioSpec
+      (.yield (.join k) (toks.map .inr) outputs) .τ
+  | spec_input {tok vals} :
+    tok ≡ ioSpec.pre vals →
+    Guard opSpec ioSpec
+      (.input ((vals.map .inl).push (.inr tok))) (.input vals)
+  | spec_output :
+    tok ≡ ioSpec.post vals →
+    Guard opSpec ioSpec
+      (.output ((vals.map .inl).push (.inr tok))) (.output vals)
+  | spec_tau :
+    Guard opSpec ioSpec .τ .τ
+
+instance
+  [Arity Op] [PCM T]
+  {opSpec : OpSpec Op V T}
+  {ioSpec : IOSpec V T m n} : LawfulLabelGuard (opSpec.Guard ioSpec) where
+  label_guard_tau := .spec_tau
+  label_guard_tau_only h := by cases h; rfl
+  label_guard_input h := by cases h; simp
+  label_guard_output h := by cases h; simp
+  label_guard_yield h := by cases h <;> simp
+
+/--
+Same signature as `OpSpec.TrivGuard` but does not dynamically
+check the well-formedness of the tokens.
+-/
+inductive OpSpec.TrivGuard [Arity Op] [PCM T]
+  {opSpec : OpSpec Op V T} :
+  Label (WithSpec Op opSpec) (V ⊕ T) (m + 1) (n + 1) →
+  Label Op V m n → Prop where
+  | spec_yield :
+    TrivGuard
+      (.yield (.op op) ((inputs.map .inl).push tok₁) ((outputs.map .inl).push tok₂))
+      (.yield op inputs outputs)
+  | spec_join : TrivGuard (.yield (.join k) toks outputs) .τ
+  | spec_input : TrivGuard (.input ((vals.map .inl).push tok)) (.input vals)
+  | spec_output : TrivGuard (.output ((vals.map .inl).push tok)) (.output vals)
+  | spec_tau : TrivGuard .τ .τ
+
+end Wavelet.Semantics
